Splinter/Betree/LinkedBetreeRefinement.i.dfy
@@ -1166,7 +1166,6 @@ module LinkedBetreeRefinement {
         assert PivotBetree.NextStep(I(v), I(v'), ILbl(lbl), IStep(step));
       }
       case FreezeAsStep() => {
-        InternalFreezeAsStepRefines(v, v', lbl, step);
         assert PivotBetree.NextStep(I(v), I(v'), ILbl(lbl), IStep(step));
       }
       case InternalGrowStep(_) => {
